Prove reorder in while

src/opt/while/ReorderLoad.v
@@ -61,7 +61,7 @@ Inductive reorder_load r1 l1 o1: forall (i2:Instr.t), Prop :=
 
 Inductive sim_load: forall (st_src:(Language.state lang)) (lc_src:Local.t) (sc1_src:TimeMap.t) (mem1_src:Memory.t)
                       (st_tgt:(Language.state lang)) (lc_tgt:Local.t) (sc1_tgt:TimeMap.t) (mem1_tgt:Memory.t), Prop :=
-| sim_load_intro
+| sim_load_read
     r1 l1 ts1 v1 released1 o1 i2 rs
     lc1_src sc1_src mem1_src
     lc1_tgt sc1_tgt mem1_tgt
@@ -69,6 +69,24 @@ Inductive sim_load: forall (st_src:(Language.state lang)) (lc_src:Local.t) (sc1_
     (REORDER: reorder_load r1 l1 o1 i2)
     (READ: Local.read_step lc1_src mem1_src l1 ts1 v1 released1 o1 lc2_src)
     (LOCAL: sim_local SimPromises.bot lc2_src lc1_tgt)
+    (SC: TimeMap.le sc1_src sc1_tgt)
+    (MEMORY: sim_memory mem1_src mem1_tgt)
+    (WF_SRC: Local.wf lc1_src mem1_src)
+    (WF_TGT: Local.wf lc1_tgt mem1_tgt)
+    (SC_SRC: Memory.closed_timemap sc1_src mem1_src)
+    (SC_TGT: Memory.closed_timemap sc1_tgt mem1_tgt)
+    (MEM_SRC: Memory.closed mem1_src)
+    (MEM_TGT: Memory.closed mem1_tgt):
+    sim_load
+      (State.mk rs [Stmt.instr i2; Stmt.instr (Instr.load r1 l1 o1)]) lc1_src sc1_src mem1_src
+      (State.mk (RegFun.add r1 v1 rs) [Stmt.instr i2]) lc1_tgt sc1_tgt mem1_tgt
+| sim_load_racy_read
+    r1 l1 v1 o1 i2 rs
+    lc1_src sc1_src mem1_src
+    lc1_tgt sc1_tgt mem1_tgt
+    (REORDER: reorder_load r1 l1 o1 i2)
+    (READ: Local.racy_read_step lc1_src mem1_src l1 v1 o1)
+    (LOCAL: sim_local SimPromises.bot lc1_src lc1_tgt)
     (SC: TimeMap.le sc1_src sc1_tgt)
     (MEMORY: sim_memory mem1_src mem1_tgt)
     (WF_SRC: Local.wf lc1_src mem1_src)
@@ -88,7 +106,7 @@ Lemma sim_load_sim_local
       (SIM: sim_load st_src lc_src sc_src mem_src st_tgt lc_tgt sc_tgt mem_tgt):
   sim_local SimPromises.bot lc_src lc_tgt.
 Proof.
-  inv SIM.
+  inv SIM; eauto.
   exploit Local.read_step_future; eauto. i. des.
   inv READ. inv LOCAL. ss.
   econs; eauto. etrans; eauto.
@@ -116,8 +134,11 @@ Lemma sim_load_mon
   sim_load st_src lc_src sc2_src mem2_src
            st_tgt lc_tgt sc2_tgt mem2_tgt.
 Proof.
-  inv SIM1. exploit future_read_step; try exact READ; eauto. i. des.
-  econs; eauto. etrans; eauto.
+  inv SIM1.
+  - exploit future_read_step; try exact READ; eauto. i. des.
+    econs; eauto. etrans; eauto.
+  - exploit future_racy_read_step; try exact READ; eauto. i. des.
+    econs 2; eauto.
 Qed.
 
 Lemma sim_load_step
@@ -130,185 +151,363 @@ Lemma sim_load_step
                    st1_tgt lc1_tgt sc1_tgt mem1_tgt.
 Proof.
   exploit sim_load_sim_local; eauto. intro SIM_LC.
-  inv SIM. ii.
-  exploit Local.read_step_future; eauto. i. des.
-  inv STEP_TGT; [inv STEP|inv STEP; inv LOCAL0];
-    try (inv STATE; inv INSTR; inv REORDER); ss.
-  - (* promise *)
-    right.
-    exploit Local.promise_step_future; eauto. i. des.
-    exploit sim_local_promise_bot; eauto. i. des.
-    exploit reorder_read_promise; try exact READ; try exact STEP_SRC; eauto. i. des.
-    exploit Local.promise_step_future; eauto. i. des.
-    esplits; try apply SC; eauto; ss.
-    + econs 2. econs. econs; eauto.
-    + eauto.
-    + right. econs; eauto. etrans; eauto.
-  - (* load *)
-    right.
-    exploit sim_local_read; (try by etrans; eauto); eauto; try refl. i. des.
-    exploit reorder_read_read; try exact READ; try exact STEP_SRC; eauto. i. des.
-    esplits.
-    + ss.
-    + econs 2; [|econs 1]. econs.
-      * econs. econs 2. econs; [|econs 2]; eauto. econs. econs.
-      * eauto.
-    + econs 2. econs 2. econs; [|econs 2]; eauto. econs. econs.
-    + eauto.
-    + eauto.
-    + eauto.
-    + left. eapply paco11_mon; [apply sim_stmts_nil|]; ss.
-      apply RegFun.add_add. ii. subst. eapply REGS.
-      * apply RegSet.singleton_spec. eauto.
-      * apply RegSet.singleton_spec. eauto.
-  - (* update-load *)
-    right.
-    guardH ORDW2.
-    exploit sim_local_read; (try by etrans; eauto); eauto; try refl. i. des.
-    exploit reorder_read_read; try exact READ; try exact STEP_SRC; try by eauto. i. des.
-    esplits.
-    + ss.
-    + econs 2; [|econs 1]. econs.
-      * econs. econs 2. econs; [|econs 2]; eauto. econs. econs.
+  inv SIM.
+  { (* read *)
+    ii.
+    exploit Local.read_step_future; eauto. i. des.
+    inv STEP_TGT; [inv STEP|inv STEP; inv LOCAL0];
+      try (inv STATE; inv INSTR; inv REORDER); ss.
+    - (* promise *)
+      right.
+      exploit Local.promise_step_future; eauto. i. des.
+      exploit sim_local_promise_bot; eauto. i. des.
+      exploit reorder_read_promise; try exact READ; try exact STEP_SRC; eauto. i. des.
+      exploit Local.promise_step_future; eauto. i. des.
+      esplits; try apply SC; eauto; ss.
+      + econs 2. econs. econs; eauto.
+      + eauto.
+      + right. econs; eauto. etrans; eauto.
+    - (* load *)
+      right.
+      exploit sim_local_read; (try by etrans; eauto); eauto; try refl. i. des.
+      exploit reorder_read_read; try exact READ; try exact STEP_SRC; eauto. i. des.
+      esplits.
+      + ss.
+      + econs 2; [|econs 1]. econs.
+        * econs. econs 2. econs; [|econs 2]; eauto. econs. econs.
+        * eauto.
+      + econs 2. econs 2. econs; [|econs 2]; eauto. econs. econs.
+      + eauto.
+      + eauto.
+      + eauto.
+      + left. eapply paco11_mon; [apply sim_stmts_nil|]; ss.
+        apply RegFun.add_add. ii. subst. eapply REGS.
+        * apply RegSet.singleton_spec. eauto.
+        * apply RegSet.singleton_spec. eauto.
+    - (* update-load *)
+      right.
+      guardH ORDW2.
+      exploit sim_local_read; (try by etrans; eauto); eauto; try refl. i. des.
+      exploit reorder_read_read; try exact READ; try exact STEP_SRC; try by eauto. i. des.
+      esplits.
+      + ss.
+      + econs 2; [|econs 1]. econs.
+        * econs. econs 2. econs; [|econs 2]; eauto. econs. econs.
+          erewrite <- RegFile.eq_except_rmw; eauto; try apply RegFile.eq_except_singleton.
+          ii. eapply REGS; eauto.
+          apply RegSet.singleton_spec in LHS. subst.
+          apply RegSet.add_spec. auto.
+        * eauto.
+      + econs 2. econs 2. econs; [|econs 2]; eauto. econs. econs.
+      + eauto.
+      + eauto.
+      + eauto.
+      + left. eapply paco11_mon; [apply sim_stmts_nil|]; ss.
+        apply RegFun.add_add. ii. subst. eapply REGS.
+        * apply RegSet.singleton_spec. eauto.
+        * apply RegSet.add_spec. auto.
+    - (* store *)
+      right.
+      guardH ORD.
+      hexploit sim_local_write_bot; try exact LOCAL1; try exact SC;
+        try exact WF2; try refl; eauto; try by viewtac. i. des.
+      exploit reorder_read_write; try exact READ; try exact STEP_SRC; eauto; try by viewtac. i. des.
+      esplits.
+      + ss.
+      + econs 2; [|econs 1]. econs.
+        * econs. econs 2. econs; [|econs 3]; eauto. econs.
+          erewrite RegFile.eq_except_value; eauto.
+          { econs. }
+          { apply RegFile.eq_except_singleton. }
+        * eauto.
+      + econs 2. econs 2. econs; [|econs 2]; eauto. econs. econs.
+      + eauto.
+      + eauto.
+      + etrans; eauto.
+      + left. eapply paco11_mon; [apply sim_stmts_nil|]; ss. etrans; eauto.
+    - (* update *)
+      right.
+      guardH ORDW2.
+      exploit Local.read_step_future; try exact LOCAL1; eauto. i. des.
+      exploit sim_local_read; try exact LOCAL1; eauto; try refl. i. des.
+      exploit Local.read_step_future; try exact STEP_SRC; eauto. i. des.
+      hexploit sim_local_write_bot; try exact LOCAL2; try exact SC; eauto; try refl. i. des.
+      exploit reorder_read_read; try exact READ; try exact STEP_SRC; eauto; try congr. i. des.
+      exploit Local.read_step_future; try exact STEP1; eauto. i. des.
+      exploit reorder_read_write; try exact STEP2; try exact STEP_SRC0; eauto; try congr. i. des.
+      esplits.
+      + ss.
+      + econs 2; [|econs 1]. econs.
+        * econs. econs 2. econs; [|econs 4]; eauto. econs. econs.
+          erewrite <- RegFile.eq_except_rmw; eauto; try apply RegFile.eq_except_singleton.
+          ii. eapply REGS; eauto.
+          apply RegSet.singleton_spec in LHS. subst.
+          apply RegSet.add_spec. auto.
+        * eauto.
+      + econs 2. econs 2. econs; [|econs 2]; eauto. econs. econs.
+      + eauto.
+      + eauto.
+      + etrans; eauto.
+      + left. eapply paco11_mon; [apply sim_stmts_nil|]; ss.
+        * apply RegFun.add_add. ii. subst. eapply REGS.
+          { apply RegSet.singleton_spec. eauto. }
+          { apply RegSet.add_spec. eauto. }
+        * etrans; eauto.
+    - (* fence *)
+      right.
+      exploit sim_local_fence; try exact LOCAL1; try exact SC; eauto; try refl. i. des.
+      exploit reorder_read_fence; try exact READ; try exact STEP_SRC; eauto. i. des.
+      esplits.
+      + ss.
+      + econs 2; [|econs 1]. econs.
+        * econs. econs 2. econs; [|econs 5]; eauto. econs. econs.
+        * eauto.
+      + econs 2. econs 2. econs; [|econs 2]; eauto. econs. econs.
+      + eauto.
+      + etrans; eauto.
+      + eauto.
+      + left. eapply paco11_mon; [apply sim_stmts_nil|]; ss.
+        etrans; eauto.
+    - (* na write *)
+      inv LOCAL1. destruct ord; ss.
+    - (* racy read *)
+      right.
+      exploit sim_local_racy_read; try exact LOCAL; eauto; try refl. i. des.
+      exploit reorder_read_racy_read; try exact READ; try exact x0; eauto. i. des.
+      esplits.
+      + ss.
+      + econs 2; [|econs 1]. econs.
+        * econs. econs 2. econs; [|econs 9]; eauto. econs. econs.
+        * eauto.
+      + econs 2. econs 2. econs; [|econs 2]; eauto. econs. econs.
+      + eauto.
+      + eauto.
+      + eauto.
+      + left. eapply paco11_mon; [apply sim_stmts_nil|]; ss.
+        apply RegFun.add_add. ii. subst. eapply REGS.
+        * apply RegSet.singleton_spec. eauto.
+        * apply RegSet.singleton_spec. eauto.
+    - (* racy read *)
+      right. guardH ORDW2.
+      exploit sim_local_racy_read; try exact LOCAL; eauto; try refl. i. des.
+      exploit reorder_read_racy_read; try exact READ; try exact x0; eauto; ss. i. des.
+      esplits.
+      + ss.
+      + econs 2; [|econs 1]. econs.
+        * econs. econs 2. econs; [|econs 9]; eauto. econs. econs.
+          erewrite <- RegFile.eq_except_rmw; eauto; try apply RegFile.eq_except_singleton.
+          ii. eapply REGS; eauto.
+          apply RegSet.singleton_spec in LHS. subst.
+          apply RegSet.add_spec. auto.
+        * eauto.
+      + econs 2. econs 2. econs; [|econs 2]; eauto. econs. econs.
+      + eauto.
+      + eauto.
+      + eauto.
+      + left. eapply paco11_mon; [apply sim_stmts_nil|]; ss.
+        apply RegFun.add_add. ii. subst. eapply REGS.
+        * apply RegSet.singleton_spec. eauto.
+        * apply RegSet.add_spec. auto.
+    - (* racy write *)
+      left. guardH ORD.
+      exploit sim_local_racy_write; try exact LOCAL1; try exact SIM_LC;
+        try match goal with
+            | [|- is_true (Ordering.le _ _)] => refl
+            end; eauto.
+      i. des.
+      unfold Thread.steps_failure. esplits; try refl.
+      + econs 2. econs; [|econs 10]; eauto. econs. econs.
+      + ss.
+    - (* racy update *)
+      left. guardH ORDW2.
+      exploit sim_local_racy_update; try exact LOCAL1; try exact SIM_LC;
+        try match goal with
+            | [|- is_true (Ordering.le _ _)] => refl
+            end; eauto.
+      i. des.
+      unfold Thread.steps_failure. esplits; try refl.
+      + econs 2. econs; [|econs 11]; eauto. econs. econs.
         erewrite <- RegFile.eq_except_rmw; eauto; try apply RegFile.eq_except_singleton.
         ii. eapply REGS; eauto.
         apply RegSet.singleton_spec in LHS. subst.
         apply RegSet.add_spec. auto.
-      * eauto.
-    + econs 2. econs 2. econs; [|econs 2]; eauto. econs. econs.
-    + eauto.
-    + eauto.
-    + eauto.
-    + left. eapply paco11_mon; [apply sim_stmts_nil|]; ss.
-      apply RegFun.add_add. ii. subst. eapply REGS.
-      * apply RegSet.singleton_spec. eauto.
-      * apply RegSet.add_spec. auto.
-  - (* store *)
-    right.
-    guardH ORD.
-    hexploit sim_local_write_bot; try exact LOCAL1; try exact SC;
-      try exact WF2; try refl; eauto; try by viewtac. i. des.
-    exploit reorder_read_write; try exact READ; try exact STEP_SRC; eauto; try by viewtac. i. des.
-    esplits.
-    + ss.
-    + econs 2; [|econs 1]. econs.
-      * econs. econs 2. econs; [|econs 3]; eauto. econs.
-        erewrite RegFile.eq_except_value; eauto.
-        { econs. }
-        { apply RegFile.eq_except_singleton. }
-      * eauto.
-    + econs 2. econs 2. econs; [|econs 2]; eauto. econs. econs.
-    + eauto.
-    + eauto.
-    + etrans; eauto.
-    + left. eapply paco11_mon; [apply sim_stmts_nil|]; ss. etrans; eauto.
-  - (* update *)
-    right.
-    guardH ORDW2.
-    exploit Local.read_step_future; try exact LOCAL1; eauto. i. des.
-    exploit sim_local_read; try exact LOCAL1; eauto; try refl. i. des.
-    exploit Local.read_step_future; try exact STEP_SRC; eauto. i. des.
-    hexploit sim_local_write_bot; try exact LOCAL2; try exact SC; eauto; try refl. i. des.
-    exploit reorder_read_read; try exact READ; try exact STEP_SRC; eauto; try congr. i. des.
-    exploit Local.read_step_future; try exact STEP1; eauto. i. des.
-    exploit reorder_read_write; try exact STEP2; try exact STEP_SRC0; eauto; try congr. i. des.
-    esplits.
-    + ss.
-    + econs 2; [|econs 1]. econs.
-      * econs. econs 2. econs; [|econs 4]; eauto. econs. econs.
-        erewrite <- RegFile.eq_except_rmw; eauto; try apply RegFile.eq_except_singleton.
-        ii. eapply REGS; eauto.
-        apply RegSet.singleton_spec in LHS. subst.
-        apply RegSet.add_spec. auto.
-      * eauto.
-    + econs 2. econs 2. econs; [|econs 2]; eauto. econs. econs.
-    + eauto.
-    + eauto.
-    + etrans; eauto.
-    + left. eapply paco11_mon; [apply sim_stmts_nil|]; ss.
-      * apply RegFun.add_add. ii. subst. eapply REGS.
+      + ss.
+  }
+
+  { (* racy read *)
+    ii.
+    inv STEP_TGT; [inv STEP|inv STEP; inv LOCAL0];
+      try (inv STATE; inv INSTR; inv REORDER); ss.
+    - (* promise *)
+      right.
+      exploit Local.promise_step_future; eauto. i. des.
+      exploit sim_local_promise_bot; eauto. i. des.
+      exploit reorder_racy_read_promise; try exact READ; try exact STEP_SRC; eauto. i. des.
+      exploit Local.promise_step_future; try exact STEP_SRC; eauto. i. des.
+      esplits; try apply SC; eauto; ss.
+      + econs 2. econs. econs; eauto.
+      + eauto.
+      + right. econs 2; eauto.
+    - (* load *)
+      right.
+      exploit sim_local_read; (try by etrans; eauto); eauto; try refl. i. des.
+      exploit reorder_racy_read_read; try exact READ; try exact STEP_SRC; eauto. i. des.
+      esplits.
+      + ss.
+      + econs 2; [|econs 1]. econs.
+        * econs. econs 2. econs; [|econs 2]; eauto. econs. econs.
+        * eauto.
+      + econs 2. econs 2. econs; [|econs 9]; eauto. econs. econs.
+      + eauto.
+      + eauto.
+      + eauto.
+      + left. eapply paco11_mon; [apply sim_stmts_nil|]; ss.
+        apply RegFun.add_add. ii. subst. eapply REGS.
+        * apply RegSet.singleton_spec. eauto.
+        * apply RegSet.singleton_spec. eauto.
+    - (* update-load *)
+      right.
+      guardH ORDW2.
+      exploit sim_local_read; (try by etrans; eauto); eauto; try refl. i. des.
+      exploit reorder_racy_read_read; try exact READ; try exact STEP_SRC; try by eauto. i. des.
+      esplits.
+      + ss.
+      + econs 2; [|econs 1]. econs.
+        * econs. econs 2. econs; [|econs 2]; eauto. econs. econs.
+          erewrite <- RegFile.eq_except_rmw; eauto; try apply RegFile.eq_except_singleton.
+          ii. eapply REGS; eauto.
+          apply RegSet.singleton_spec in LHS. subst.
+          apply RegSet.add_spec. auto.
+        * eauto.
+      + econs 2. econs 2. econs; [|econs 9]; eauto. econs. econs.
+      + eauto.
+      + eauto.
+      + eauto.
+      + left. eapply paco11_mon; [apply sim_stmts_nil|]; ss.
+        apply RegFun.add_add. ii. subst. eapply REGS.
+        * apply RegSet.singleton_spec. eauto.
+        * apply RegSet.add_spec. auto.
+    - (* store *)
+      right.
+      guardH ORD.
+      hexploit sim_local_write_bot; try exact LOCAL1; try exact SC;
+        try exact WF_SRC; try exact WF_TGT; try refl; eauto; try by viewtac. i. des.
+      exploit reorder_racy_read_write; try exact READ; eauto. i. des.
+      esplits.
+      + ss.
+      + econs 2; [|econs 1]. econs.
+        * econs. econs 2. econs; [|econs 3]; eauto. econs.
+          erewrite RegFile.eq_except_value; eauto.
+          { econs. }
+          { apply RegFile.eq_except_singleton. }
+        * eauto.
+      + econs 2. econs 2. econs; [|econs 9]; eauto. econs. econs.
+      + eauto.
+      + eauto.
+      + ss.
+      + left. eapply paco11_mon; [apply sim_stmts_nil|]; ss.
+    - (* update *)
+      right.
+      guardH ORDW2.
+      exploit Local.read_step_future; try exact LOCAL1; eauto. i. des.
+      exploit sim_local_read; try exact LOCAL1; eauto; try refl. i. des.
+      exploit Local.read_step_future; try exact STEP_SRC; eauto. i. des.
+      hexploit sim_local_write_bot; try exact LOCAL2; try exact SC; eauto; try refl. i. des.
+      exploit reorder_racy_read_update; try exact READ; eauto. i. des.
+      esplits.
+      + ss.
+      + econs 2; [|econs 1]. econs.
+        * econs. econs 2. econs; [|econs 4]; eauto. econs. econs.
+          erewrite <- RegFile.eq_except_rmw; eauto; try apply RegFile.eq_except_singleton.
+          ii. eapply REGS; eauto.
+          apply RegSet.singleton_spec in LHS. subst.
+          apply RegSet.add_spec. auto.
+        * eauto.
+      + econs 2. econs 2. econs; [|econs 9]; eauto. econs. econs.
+      + eauto.
+      + eauto.
+      + ss.
+      + left. eapply paco11_mon; [apply sim_stmts_nil|]; ss.
+        apply RegFun.add_add. ii. subst. eapply REGS.
         { apply RegSet.singleton_spec. eauto. }
         { apply RegSet.add_spec. eauto. }
-      * etrans; eauto.
-  - (* fence *)
-    right.
-    exploit sim_local_fence; try exact LOCAL1; try exact SC; eauto; try refl. i. des.
-    exploit reorder_read_fence; try exact READ; try exact STEP_SRC; eauto. i. des.
-    esplits.
-    + ss.
-    + econs 2; [|econs 1]. econs.
-      * econs. econs 2. econs; [|econs 5]; eauto. econs. econs.
-      * eauto.
-    + econs 2. econs 2. econs; [|econs 2]; eauto. econs. econs.
-    + eauto.
-    + etrans; eauto.
-    + eauto.
-    + left. eapply paco11_mon; [apply sim_stmts_nil|]; ss.
-      etrans; eauto.
-  - (* na write *)
-    inv LOCAL1. destruct ord; ss.
-  - (* racy read *)
-    right.
-    exploit sim_local_racy_read; try exact LOCAL; eauto; try refl. i. des.
-    exploit reorder_read_racy_read; try exact READ; try exact x0; eauto. i. des.
-    esplits.
-    + ss.
-    + econs 2; [|econs 1]. econs.
-      * econs. econs 2. econs; [|econs 9]; eauto. econs. econs.
-      * eauto.
-    + econs 2. econs 2. econs; [|econs 2]; eauto. econs. econs.
-    + eauto.
-    + eauto.
-    + eauto.
-    + left. eapply paco11_mon; [apply sim_stmts_nil|]; ss.
-      apply RegFun.add_add. ii. subst. eapply REGS.
-      * apply RegSet.singleton_spec. eauto.
-      * apply RegSet.singleton_spec. eauto.
-  - (* racy read *)
-    right. guardH ORDW2.
-    exploit sim_local_racy_read; try exact LOCAL; eauto; try refl. i. des.
-    exploit reorder_read_racy_read; try exact READ; try exact x0; eauto; ss. i. des.
-    esplits.
-    + ss.
-    + econs 2; [|econs 1]. econs.
-      * econs. econs 2. econs; [|econs 9]; eauto. econs. econs.
+    - (* fence *)
+      right.
+      exploit sim_local_fence; try exact LOCAL1; try exact SC; eauto; try refl. i. des.
+      exploit reorder_racy_read_fence; try exact READ; try exact STEP_SRC; eauto. i. des.
+      esplits.
+      + ss.
+      + econs 2; [|econs 1]. econs.
+        * econs. econs 2. econs; [|econs 5]; eauto. econs. econs.
+        * eauto.
+      + econs 2. econs 2. econs; [|econs 9]; eauto. econs. econs.
+      + eauto.
+      + ss.
+      + eauto.
+      + left. eapply paco11_mon; [apply sim_stmts_nil|]; ss.
+    - (* na write *)
+      inv LOCAL1. destruct ord; ss.
+    - (* racy read *)
+      right.
+      exploit sim_local_racy_read; try exact LOCAL; eauto; try refl. i. des.
+      esplits.
+      + ss.
+      + econs 2; [|econs 1]. econs.
+        * econs. econs 2. econs; [|econs 9]; eauto. econs. econs.
+        * eauto.
+      + econs 2. econs 2. econs; [|econs 9]; try exact READ. econs. econs.
+      + eauto.
+      + eauto.
+      + eauto.
+      + left. eapply paco11_mon; [apply sim_stmts_nil|]; ss.
+        apply RegFun.add_add. ii. subst. eapply REGS.
+        * apply RegSet.singleton_spec. eauto.
+        * apply RegSet.singleton_spec. eauto.
+    - (* racy read *)
+      right. guardH ORDW2.
+      exploit sim_local_racy_read; try exact LOCAL; eauto; try refl. i. des.
+      esplits.
+      + ss.
+      + econs 2; [|econs 1]. econs.
+        * econs. econs 2. econs; [|econs 9]; eauto. econs. econs.
+          erewrite <- RegFile.eq_except_rmw; eauto; try apply RegFile.eq_except_singleton.
+          ii. eapply REGS; eauto.
+          apply RegSet.singleton_spec in LHS. subst.
+          apply RegSet.add_spec. auto.
+        * eauto.
+      + econs 2. econs 2. econs; [|econs 9]; try exact READ. econs. econs.
+      + eauto.
+      + eauto.
+      + eauto.
+      + left. eapply paco11_mon; [apply sim_stmts_nil|]; ss.
+        apply RegFun.add_add. ii. subst. eapply REGS.
+        * apply RegSet.singleton_spec. eauto.
+        * apply RegSet.add_spec. auto.
+    - (* racy write *)
+      left. guardH ORD.
+      exploit sim_local_racy_write; try exact LOCAL1; try exact SIM_LC;
+        try match goal with
+            | [|- is_true (Ordering.le _ _)] => refl
+            end; eauto.
+      i. des.
+      unfold Thread.steps_failure. esplits; try refl.
+      + econs 2. econs; [|econs 10]; eauto. econs. econs.
+      + ss.
+    - (* racy update *)
+      left. guardH ORDW2.
+      exploit sim_local_racy_update; try exact LOCAL1; try exact SIM_LC;
+        try match goal with
+            | [|- is_true (Ordering.le _ _)] => refl
+            end; eauto.
+      i. des.
+      unfold Thread.steps_failure. esplits; try refl.
+      + econs 2. econs; [|econs 11]; eauto. econs. econs.
         erewrite <- RegFile.eq_except_rmw; eauto; try apply RegFile.eq_except_singleton.
         ii. eapply REGS; eauto.
         apply RegSet.singleton_spec in LHS. subst.
         apply RegSet.add_spec. auto.
-      * eauto.
-    + econs 2. econs 2. econs; [|econs 2]; eauto. econs. econs.
-    + eauto.
-    + eauto.
-    + eauto.
-    + left. eapply paco11_mon; [apply sim_stmts_nil|]; ss.
-      apply RegFun.add_add. ii. subst. eapply REGS.
-      * apply RegSet.singleton_spec. eauto.
-      * apply RegSet.add_spec. auto.
-  - (* racy write *)
-    left. guardH ORD.
-    exploit sim_local_racy_write; try exact LOCAL1; try exact SIM_LC;
-      try match goal with
-          | [|- is_true (Ordering.le _ _)] => refl
-          end; eauto.
-    i. des.
-    unfold Thread.steps_failure. esplits; try refl.
-    + econs 2. econs; [|econs 10]; eauto. econs. econs.
-    + ss.
-  - (* racy update *)
-    left. guardH ORDW2.
-    exploit sim_local_racy_update; try exact LOCAL1; try exact SIM_LC;
-      try match goal with
-          | [|- is_true (Ordering.le _ _)] => refl
-          end; eauto.
-    i. des.
-    unfold Thread.steps_failure. esplits; try refl.
-    + econs 2. econs; [|econs 11]; eauto. econs. econs.
-      erewrite <- RegFile.eq_except_rmw; eauto; try apply RegFile.eq_except_singleton.
-      ii. eapply REGS; eauto.
-      apply RegSet.singleton_spec in LHS. subst.
-      apply RegSet.add_spec. auto.
-    + ss.
+      + ss.
+  }
 Qed.
 
 Lemma sim_load_sim_thread:
@@ -317,9 +516,11 @@ Proof.
   pcofix CIH. i. pfold. ii. ss. splits; ss; ii.
   - inv TERMINAL_TGT. inv PR; ss.
   - right.
-    esplits; eauto.
-    inv PR. inv READ. inv LOCAL. ss.
-    apply SimPromises.sem_bot_inv in PROMISES; auto. rewrite PROMISES. auto.
+    esplits; eauto. inv PR.
+    + inv READ. inv LOCAL. ss.
+      apply SimPromises.sem_bot_inv in PROMISES; auto. rewrite PROMISES. auto.
+    + inv READ. inv LOCAL. ss.
+      apply SimPromises.sem_bot_inv in PROMISES; auto. rewrite PROMISES. auto.
   - exploit sim_load_mon; eauto. i.
     exploit sim_load_step; eauto. i. des; eauto.
     + right. esplits; eauto.
