src/opt/while/ReorderUpdate.v
@@ -16,6 +16,7 @@ Require Import Configuration.
 Require Import Progress.
 
 Require Import FulfillStep.
+Require Import LowerPromises.
 
 Require Import SimMemory.
 Require Import SimPromises.
@@ -25,6 +26,7 @@ Require Import Compatibility.
 
 Require Import ReorderStep.
 Require Import ProgressStep.
+Require Import ReorderAbortCommon.
 
 Require Import Syntax.
 Require Import Semantics.
@@ -64,7 +66,7 @@ Inductive reorder_update r1 l1 rmw1 or1 ow1: forall (i2:Instr.t), Prop :=
 
 Inductive sim_update: forall (st_src:(Language.state lang)) (lc_src:Local.t) (sc1_src:TimeMap.t) (mem1_src:Memory.t)
                         (st_tgt:(Language.state lang)) (lc_tgt:Local.t) (sc1_tgt:TimeMap.t) (mem1_tgt:Memory.t), Prop :=
-| sim_update_intro
+| sim_update_update
     r1 l1 from1 to1 vr1 vret1 vw1 releasedr1 releasedw1 rmw1 or1 ow1 i2 rs
     lc1_src sc1_src mem1_src
     lc1_tgt sc1_tgt mem1_tgt
@@ -79,6 +81,28 @@ Inductive sim_update: forall (st_src:(Language.state lang)) (lc_src:Local.t) (sc
               end)
     (LOCAL: sim_local SimPromises.bot lc3_src lc1_tgt)
     (SC: TimeMap.le sc3_src sc1_tgt)
+    (MEMORY: sim_memory mem1_src mem1_tgt)
+    (WF_SRC: Local.wf lc1_src mem1_src)
+    (WF_TGT: Local.wf lc1_tgt mem1_tgt)
+    (SC_SRC: Memory.closed_timemap sc1_src mem1_src)
+    (SC_TGT: Memory.closed_timemap sc1_tgt mem1_tgt)
+    (MEM_SRC: Memory.closed mem1_src)
+    (MEM_TGT: Memory.closed mem1_tgt):
+    sim_update
+      (State.mk rs [Stmt.instr i2; Stmt.instr (Instr.update r1 l1 rmw1 or1 ow1)]) lc1_src sc1_src mem1_src
+      (State.mk (RegFun.add r1 vret1 rs) [Stmt.instr i2]) lc1_tgt sc1_tgt mem1_tgt
+| sim_update_racy_update
+    r1 l1 vr1 vret1 vw1 rmw1 or1 ow1 i2 rs
+    lc1_src sc1_src mem1_src
+    lc1_tgt sc1_tgt mem1_tgt
+    (RMW: RegFile.eval_rmw rs rmw1 vr1 = (vret1, vw1))
+    (REORDER: reorder_update r1 l1 rmw1 or1 ow1 i2)
+    (RACY_UPDATE: match vw1 with
+                  | Some val => Local.racy_update_step lc1_src mem1_src l1 or1 ow1
+                  | None => Local.racy_read_step lc1_src mem1_src l1 vr1 or1
+                  end)
+    (LOCAL: sim_local SimPromises.bot lc1_src lc1_tgt)
+    (SC: TimeMap.le sc1_src sc1_tgt)
     (MEMORY: sim_memory mem1_src mem1_tgt)
     (WF_SRC: Local.wf lc1_src mem1_src)
     (WF_TGT: Local.wf lc1_tgt mem1_tgt)
@@ -114,23 +138,28 @@ Lemma sim_update_mon
              st_tgt lc_tgt sc2_tgt mem2_tgt.
 Proof.
   inv SIM1.
-  exploit Local.read_step_future; eauto. i. des.
-  exploit future_read_step; try exact READ; eauto. i. des.
-  exploit Local.read_step_future; eauto. i. des.
-  destruct vw1 as [vw1|]; cycle 1.
-  { ss; des; subst. econs; [eauto|..]; s; eauto; etrans; eauto. }
-  exploit future_fulfill_step; try exact FULFILL; eauto. i. des.
-  exploit sim_local_fulfill_bot; try apply x0; try exact LOCAL0; try refl;
-    try exact WF0; try by viewtac.
-  { econs.
-    - apply WF2.
-    - eapply TView.future_weak_closed; eauto. apply WF2.
-    - inv READ. apply WF_SRC.
-    - apply WF2.
-    - apply WF2.
-  }
-  i. des.
-  econs; [eauto|..]; s; eauto; etrans; eauto.
+  - exploit Local.read_step_future; eauto. i. des.
+    exploit future_read_step; try exact READ; eauto. i. des.
+    exploit Local.read_step_future; eauto. i. des.
+    destruct vw1 as [vw1|]; cycle 1.
+    { ss; des; subst. econs; [eauto|..]; s; eauto; etrans; eauto. }
+    exploit future_fulfill_step; try exact FULFILL; eauto. i. des.
+    exploit sim_local_fulfill_bot; try apply x0; try exact LOCAL0; try refl;
+      try exact WF0; try by viewtac.
+    { econs.
+      - apply WF2.
+      - eapply TView.future_weak_closed; eauto. apply WF2.
+      - inv READ. apply WF_SRC.
+      - apply WF2.
+      - apply WF2.
+    }
+    i. des.
+    econs; [eauto|..]; s; eauto; etrans; eauto.
+  - destruct vw1 as [vw1|].
+    + exploit future_racy_update_step; try exact RACY_UPDATE; eauto. i. des.
+      econs 2; eauto.
+    + exploit future_racy_read_step; try exact RACY_UPDATE; eauto. i. des.
+      econs 2; eauto.
 Grab Existential Variables.
 { econs 2. }
 { econs. econs 3. }
@@ -145,208 +174,360 @@ Lemma sim_update_step
                    st1_src lc1_src sc1_src mem1_src
                    st1_tgt lc1_tgt sc1_tgt mem1_tgt.
 Proof.
-  inv SIM. ii.
-  exploit Local.read_step_future; eauto. i. des.
-  destruct vw1 as [vw1|]; cycle 1.
-  { ss. des. subst.
-    inv STEP_TGT; [inv STEP|inv STEP; inv LOCAL0];
-      try (inv STATE; inv INSTR; inv REORDER); ss.
-    - (* promise *)
-      right.
-      exploit Local.promise_step_future; eauto. i. des.
-      exploit sim_local_promise_bot; eauto. i. des.
-      exploit reorder_read_promise; try exact READ; try exact STEP_SRC; eauto. i. des.
-      exploit Local.promise_step_future; eauto. i. des.
-      esplits; try apply SC; eauto.
-      + ss.
-      + econs 2. econs. econs; eauto.
-      + eauto.
-      + right. econs; [eauto|..]; s; eauto. etrans; eauto.
-    - (* load *)
-      right.
-      exploit sim_local_read; (try by etrans; eauto); eauto; try refl. i. des.
-      exploit reorder_read_read; try exact READ; try exact STEP_SRC; try by eauto. i. des.
-      esplits.
-      + ss.
-      + econs 2; [|econs 1]. econs.
-        * econs. econs 2. econs; [|econs 2]; eauto. econs. econs.
-        * eauto.
-      + econs 2. econs 2. econs; [|econs 2]; eauto. econs. econs.
-        erewrite RegFile.eq_except_rmw; eauto; cycle 1.
-        * apply RegFile.eq_except_singleton.
-        * ii. eapply REGS; eauto.
-          apply RegSet.add_spec. auto.
-      + eauto.
-      + eauto.
-      + eauto.
-      + left. eapply paco11_mon; [apply sim_stmts_nil|]; ss.
-        apply RegFun.add_add. ii. subst. eapply REGS; cycle 1.
-        * apply RegSet.singleton_spec. eauto.
-        * apply RegSet.add_spec. auto.
-    - (* store *)
-      right.
-      guardH ORD21.
-      hexploit sim_local_write_bot; try exact LOCAL1; try exact SC;
-        try exact WF2; try refl; eauto; try by viewtac. i. des.
-      exploit reorder_read_write; try exact READ; try exact STEP_SRC; eauto; try by viewtac. i. des.
-      esplits.
-      + ss.
-      + econs 2; [|econs 1]. econs.
-        * econs. econs 2. econs; [|econs 3]; eauto. econs.
-          s. erewrite RegFile.eq_except_value; eauto. econs.
-          ii. apply RegFun.add_spec_neq. ii. subst. apply REG.
-          eapply RegSet.add_spec. auto.
-        * eauto.
-      + econs 2. econs 2. econs; [|econs 2]; eauto. econs. econs. eauto.
-      + eauto.
-      + eauto.
-      + etrans; eauto.
-      + left. eapply paco11_mon; [apply sim_stmts_nil|]; ss. etrans; eauto.
-    - (* na write *)
-      inv LOCAL1. destruct ord; ss.
-    - (* racy read *)
-      right.
-      exploit sim_local_racy_read; try exact LOCAL; eauto; try refl. i. des.
-      exploit reorder_read_racy_read; try exact READ; try exact x0; eauto; ss. i. des.
-      esplits.
-      + ss.
-      + econs 2; [|econs 1]. econs.
-        * econs. econs 2. econs; [|econs 9]; eauto. econs. econs.
-        * eauto.
-      + econs 2. econs 2. econs; [|econs 2]; eauto. econs. econs.
-        erewrite RegFile.eq_except_rmw; eauto; cycle 1.
-        * apply RegFile.eq_except_singleton.
-        * ii. eapply REGS; eauto.
-          apply RegSet.add_spec. auto.
-      + eauto.
-      + eauto.
-      + eauto.
-      + left. eapply paco11_mon; [apply sim_stmts_nil|]; ss.
-        apply RegFun.add_add. ii. subst. eapply REGS; cycle 1.
-        * apply RegSet.singleton_spec. eauto.
-        * apply RegSet.add_spec. auto.
-    - (* racy write *)
-      left. guardH ORD21.
-      assert (SIM_LC: sim_local SimPromises.bot lc1_src lc3_tgt).
-      { exploit Local.read_step_future; try exact READ; eauto. i. des.
-        inv READ. inv LOCAL. ss.
-        econs; eauto. etrans; eauto.
-      }
-      exploit sim_local_racy_write; try exact SIM_LC;
-        try match goal with
-            | [|- is_true (Ordering.le _ _)] => refl
-            end; eauto.
-      i. des.
-      unfold Thread.steps_failure. esplits; try refl.
-      + econs 2. econs; [|econs 10]; eauto. econs. econs.
-      + ss.
+  inv SIM.
+  { (* update *)
+    ii.
+    exploit Local.read_step_future; eauto. i. des.
+    destruct vw1 as [vw1|]; cycle 1.
+    { ss. des. subst.
+      inv STEP_TGT; [inv STEP|inv STEP; inv LOCAL0];
+        try (inv STATE; inv INSTR; inv REORDER); ss.
+      - (* promise *)
+        right.
+        exploit Local.promise_step_future; eauto. i. des.
+        exploit sim_local_promise_bot; eauto. i. des.
+        exploit reorder_read_promise; try exact READ; try exact STEP_SRC; eauto. i. des.
+        exploit Local.promise_step_future; eauto. i. des.
+        esplits; try apply SC; eauto.
+        + ss.
+        + econs 2. econs. econs; eauto.
+        + eauto.
+        + right. econs; [eauto|..]; s; eauto. etrans; eauto.
+      - (* load *)
+        right.
+        exploit sim_local_read; (try by etrans; eauto); eauto; try refl. i. des.
+        exploit reorder_read_read; try exact READ; try exact STEP_SRC; try by eauto. i. des.
+        esplits.
+        + ss.
+        + econs 2; [|econs 1]. econs.
+          * econs. econs 2. econs; [|econs 2]; eauto. econs. econs.
+          * eauto.
+        + econs 2. econs 2. econs; [|econs 2]; eauto. econs. econs.
+          erewrite RegFile.eq_except_rmw; eauto; cycle 1.
+          * apply RegFile.eq_except_singleton.
+          * ii. eapply REGS; eauto.
+            apply RegSet.add_spec. auto.
+        + eauto.
+        + eauto.
+        + eauto.
+        + left. eapply paco11_mon; [apply sim_stmts_nil|]; ss.
+          apply RegFun.add_add. ii. subst. eapply REGS; cycle 1.
+          * apply RegSet.singleton_spec. eauto.
+          * apply RegSet.add_spec. auto.
+      - (* store *)
+        right.
+        guardH ORD21.
+        hexploit sim_local_write_bot; try exact LOCAL1; try exact SC;
+          try exact WF2; try refl; eauto; try by viewtac. i. des.
+        exploit reorder_read_write; try exact READ; try exact STEP_SRC; eauto; try by viewtac. i. des.
+        esplits.
+        + ss.
+        + econs 2; [|econs 1]. econs.
+          * econs. econs 2. econs; [|econs 3]; eauto. econs.
+            s. erewrite RegFile.eq_except_value; eauto. econs.
+            ii. apply RegFun.add_spec_neq. ii. subst. apply REG.
+            eapply RegSet.add_spec. auto.
+          * eauto.
+        + econs 2. econs 2. econs; [|econs 2]; eauto. econs. econs. eauto.
+        + eauto.
+        + eauto.
+        + etrans; eauto.
+        + left. eapply paco11_mon; [apply sim_stmts_nil|]; ss. etrans; eauto.
+      - (* na write *)
+        inv LOCAL1. destruct ord; ss.
+      - (* racy read *)
+        right.
+        exploit sim_local_racy_read; try exact LOCAL; eauto; try refl. i. des.
+        exploit reorder_read_racy_read; try exact READ; try exact x0; eauto; ss. i. des.
+        esplits.
+        + ss.
+        + econs 2; [|econs 1]. econs.
+          * econs. econs 2. econs; [|econs 9]; eauto. econs. econs.
+          * eauto.
+        + econs 2. econs 2. econs; [|econs 2]; eauto. econs. econs.
+          erewrite RegFile.eq_except_rmw; eauto; cycle 1.
+          * apply RegFile.eq_except_singleton.
+          * ii. eapply REGS; eauto.
+            apply RegSet.add_spec. auto.
+        + eauto.
+        + eauto.
+        + eauto.
+        + left. eapply paco11_mon; [apply sim_stmts_nil|]; ss.
+          apply RegFun.add_add. ii. subst. eapply REGS; cycle 1.
+          * apply RegSet.singleton_spec. eauto.
+          * apply RegSet.add_spec. auto.
+      - (* racy write *)
+        left. guardH ORD21.
+        assert (SIM_LC: sim_local SimPromises.bot lc1_src lc3_tgt).
+        { exploit Local.read_step_future; try exact READ; eauto. i. des.
+          inv READ. inv LOCAL. ss.
+          econs; eauto. etrans; eauto.
+        }
+        exploit sim_local_racy_write; try exact SIM_LC;
+          try match goal with
+              | [|- is_true (Ordering.le _ _)] => refl
+              end; eauto.
+        i. des.
+        unfold Thread.steps_failure. esplits; try refl.
+        + econs 2. econs; [|econs 10]; eauto. econs. econs.
+        + ss.
+    }
+
+    { exploit fulfill_step_future; eauto. i. des.
+      inv STEP_TGT; [inv STEP|inv STEP; inv LOCAL0];
+        try (inv STATE; inv INSTR; inv REORDER); ss.
+      - (* promise *)
+        right.
+        exploit Local.promise_step_future; eauto. i. des.
+        exploit sim_local_promise; try apply LOCAL0; (try by etrans; eauto); eauto. i. des.
+        exploit reorder_update_promise; try exact READ; try exact FULFILL; try exact STEP_SRC; eauto. i. des.
+        exploit Local.promise_step_future; eauto. i. des.
+        esplits.
+        + ss.
+        + eauto.
+        + econs 2. econs 1. econs; eauto.
+        + auto.
+        + etrans; eauto.
+        + auto.
+        + right. econs; [eauto|..]; s; eauto.
+          * etrans; eauto.
+          * eapply Memory.future_closed_timemap; eauto.
+      - (* load *)
+        right.
+        apply RegSet.disjoint_add in REGS. des.
+        exploit sim_local_read; try apply LOCAL0; (try by etrans; eauto); eauto; try refl. i. des.
+        exploit reorder_update_read; try exact FULFILL; try exact READ; try exact STEP_SRC; eauto. i. des.
+        exploit Local.read_step_future; try exact STEP1; eauto. i. des.
+        exploit Local.read_step_future; try exact STEP2; eauto. i. des.
+        exploit fulfill_write_sim_memory; eauto. i. des.
+        esplits.
+        + ss.
+        + econs 2; eauto. econs.
+          * econs. econs 2. econs; [|econs 2]; eauto. econs. econs.
+          * auto.
+        + econs 2. econs 2. econs; [|econs 4]; eauto. econs. econs.
+          erewrite RegFile.eq_except_rmw; eauto; cycle 1.
+          * apply RegFile.eq_except_singleton.
+          * symmetry. eauto.
+        + auto.
+        + auto.
+        + etrans; eauto.
+        + left. eapply paco11_mon; [apply sim_stmts_nil|]; ss.
+          apply RegFun.add_add. ii. subst. eapply REGS.
+          apply RegSet.Facts.singleton_iff. auto.
+      - (* store *)
+        right.
+        guardH ORD21.
+        apply RegSet.disjoint_add in REGS. des.
+        hexploit sim_local_write_bot; try exact LOCAL1; try exact LOCAL; try exact SC; try exact WF0; try refl; eauto; try by viewtac. i. des.
+        hexploit reorder_update_write; try exact READ; try exact FULFILL; try exact STEP_SRC; eauto; try by viewtac.
+        { ii. subst. inv FULFILL. eapply Time.lt_strorder. eauto. }
+        i. des.
+        exploit Local.write_step_future; try exact STEP1; eauto; try by viewtac. i. des.
+        exploit Local.read_step_future; try exact STEP2; eauto; try by viewtac. i. des.
+        exploit fulfill_write_sim_memory; eauto. i. des.
+        esplits.
+        + ss.
+        + econs 2; eauto. econs.
+          * econs. econs 2. econs; [|econs 3]; eauto. econs.
+            erewrite RegFile.eq_except_value; cycle 2.
+            { apply RegFile.eq_except_singleton. }
+            { econs. }
+            { ii. apply RegSet.singleton_spec in LHS. subst. congr. }
+          * auto.
+        + econs 2. econs 2. econs; [|econs 4]; eauto. econs. econs. eauto.
+        + auto.
+        + etrans; eauto.
+        + etrans; eauto. etrans; eauto.
+        + left. eapply paco11_mon; [apply sim_stmts_nil|]; ss.
+          etrans; eauto.
+      - (* na write *)
+        inv LOCAL1. destruct ord; ss.
+      - (* racy read *)
+        right.
+        apply RegSet.disjoint_add in REGS. des.
+        exploit sim_local_racy_read; try exact LOCAL1; eauto; try refl. i. des.
+        exploit reorder_fulfill_racy_read; try exact FULFILL; eauto. i. des.
+        exploit reorder_read_racy_read; try exact READ; eauto. i. des.
+        exploit fulfill_write_sim_memory; eauto. i. des.
+        esplits.
+        + ss.
+        + econs 2; eauto. econs.
+          * econs. econs 2. econs; [|econs 9]; eauto. econs. econs.
+          * auto.
+        + econs 2. econs 2. econs; [|econs 4]; eauto. econs. econs.
+          erewrite RegFile.eq_except_rmw; eauto; cycle 1.
+          * apply RegFile.eq_except_singleton.
+          * symmetry. eauto.
+        + auto.
+        + auto.
+        + etrans; eauto.
+        + left. eapply paco11_mon; [apply sim_stmts_nil|]; ss.
+          apply RegFun.add_add. ii. subst. eapply REGS.
+          apply RegSet.Facts.singleton_iff. auto.
+      - (* racy write *)
+        left. guardH ORD21.
+        apply RegSet.disjoint_add in REGS. des.
+        exploit sim_local_racy_write; try exact LOCAL1;
+          try match goal with
+              | [|- is_true (Ordering.le _ _)] => refl
+              end; eauto. i. des.
+        exploit reorder_fulfill_racy_write; try exact FULFILL; eauto. i. des.
+        exploit reorder_read_racy_write; try exact READ; eauto. i. des.
+        unfold Thread.steps_failure.
+        esplits; try refl.
+        + econs 2. econs; [|econs 10]; eauto. econs. econs.
+        + ss.
+    }
   }
 
-  exploit fulfill_step_future; eauto. i. des.
-  inv STEP_TGT; [inv STEP|inv STEP; inv LOCAL0];
-    try (inv STATE; inv INSTR; inv REORDER); ss.
-  - (* promise *)
-    right.
-    exploit Local.promise_step_future; eauto. i. des.
-    exploit sim_local_promise; try apply LOCAL0; (try by etrans; eauto); eauto. i. des.
-    exploit reorder_update_promise; try exact READ; try exact FULFILL; try exact STEP_SRC; eauto. i. des.
-    exploit Local.promise_step_future; eauto. i. des.
-    esplits.
-    + ss.
-    + eauto.
-    + econs 2. econs 1. econs; eauto.
-    + auto.
-    + etrans; eauto.
-    + auto.
-    + right. econs; [eauto|..]; s; eauto.
-      * etrans; eauto.
-      * eapply Memory.future_closed_timemap; eauto.
-  - (* load *)
-    right.
-    apply RegSet.disjoint_add in REGS. des.
-    exploit sim_local_read; try apply LOCAL0; (try by etrans; eauto); eauto; try refl. i. des.
-    exploit reorder_update_read; try exact FULFILL; try exact READ; try exact STEP_SRC; eauto. i. des.
-    exploit Local.read_step_future; try exact STEP1; eauto. i. des.
-    exploit Local.read_step_future; try exact STEP2; eauto. i. des.
-    exploit fulfill_write_sim_memory; eauto. i. des.
-    esplits.
-    + ss.
-    + econs 2; eauto. econs.
-      * econs. econs 2. econs; [|econs 2]; eauto. econs. econs.
-      * auto.
-    + econs 2. econs 2. econs; [|econs 4]; eauto. econs. econs.
-      erewrite RegFile.eq_except_rmw; eauto; cycle 1.
-      * apply RegFile.eq_except_singleton.
-      * symmetry. eauto.
-    + auto.
-    + auto.
-    + etrans; eauto.
-    + left. eapply paco11_mon; [apply sim_stmts_nil|]; ss.
-      apply RegFun.add_add. ii. subst. eapply REGS.
-      apply RegSet.Facts.singleton_iff. auto.
-  - (* store *)
-    right.
-    guardH ORD21.
-    apply RegSet.disjoint_add in REGS. des.
-    hexploit sim_local_write_bot; try exact LOCAL1; try exact LOCAL; try exact SC; try exact WF0; try refl; eauto; try by viewtac. i. des.
-    hexploit reorder_update_write; try exact READ; try exact FULFILL; try exact STEP_SRC; eauto; try by viewtac.
-    { ii. subst. inv FULFILL. eapply Time.lt_strorder. eauto. }
-    i. des.
-    exploit Local.write_step_future; try exact STEP1; eauto; try by viewtac. i. des.
-    exploit Local.read_step_future; try exact STEP2; eauto; try by viewtac. i. des.
-    exploit fulfill_write_sim_memory; eauto. i. des.
-    esplits.
-    + ss.
-    + econs 2; eauto. econs.
-      * econs. econs 2. econs; [|econs 3]; eauto. econs.
-        erewrite RegFile.eq_except_value; cycle 2.
-        { apply RegFile.eq_except_singleton. }
-        { econs. }
-        { ii. apply RegSet.singleton_spec in LHS. subst. congr. }
-      * auto.
-    + econs 2. econs 2. econs; [|econs 4]; eauto. econs. econs. eauto.
-    + auto.
-    + etrans; eauto.
-    + etrans; eauto. etrans; eauto.
-    + left. eapply paco11_mon; [apply sim_stmts_nil|]; ss.
-      etrans; eauto.
-  - (* na write *)
-    inv LOCAL1. destruct ord; ss.
-  - (* racy read *)
-    right.
-    apply RegSet.disjoint_add in REGS. des.
-    exploit sim_local_racy_read; try exact LOCAL1; eauto; try refl. i. des.
-    exploit reorder_fulfill_racy_read; try exact FULFILL; eauto. i. des.
-    exploit reorder_read_racy_read; try exact READ; eauto. i. des.
-    exploit fulfill_write_sim_memory; eauto. i. des.
-    esplits.
-    + ss.
-    + econs 2; eauto. econs.
-      * econs. econs 2. econs; [|econs 9]; eauto. econs. econs.
-      * auto.
-    + econs 2. econs 2. econs; [|econs 4]; eauto. econs. econs.
-      erewrite RegFile.eq_except_rmw; eauto; cycle 1.
-      * apply RegFile.eq_except_singleton.
-      * symmetry. eauto.
-    + auto.
-    + auto.
-    + etrans; eauto.
-    + left. eapply paco11_mon; [apply sim_stmts_nil|]; ss.
-      apply RegFun.add_add. ii. subst. eapply REGS.
-      apply RegSet.Facts.singleton_iff. auto.
-  - (* racy write *)
-    left. guardH ORD21.
-    apply RegSet.disjoint_add in REGS. des.
-    exploit sim_local_racy_write; try exact LOCAL1;
-      try match goal with
-          | [|- is_true (Ordering.le _ _)] => refl
-          end; eauto. i. des.
-    exploit reorder_fulfill_racy_write; try exact FULFILL; eauto. i. des.
-    exploit reorder_read_racy_write; try exact READ; eauto. i. des.
-    unfold Thread.steps_failure.
-    esplits; try refl.
-    + econs 2. econs; [|econs 10]; eauto. econs. econs.
-    + ss.
+  { (* racy update *)
+    destruct vw1 as [vw1|]; cycle 1.
+    { ii. ss.
+      inv STEP_TGT; [inv STEP|inv STEP; inv LOCAL0];
+        try (inv STATE; inv INSTR; inv REORDER); ss.
+      - (* promise *)
+        right.
+        exploit Local.promise_step_future; eauto. i. des.
+        exploit sim_local_promise_bot; eauto. i. des.
+        exploit reorder_racy_read_promise; try exact RACY_UPDATE; try exact STEP_SRC; eauto. i. des.
+        exploit Local.promise_step_future; try exact STEP_SRC; eauto. i. des.
+        esplits; try apply SC; eauto; ss.
+        + econs 2. econs. econs; eauto.
+        + eauto.
+        + right. econs 2; eauto.
+      - (* load *)
+        right.
+        apply RegSet.disjoint_add in REGS. des.
+        exploit sim_local_read; (try by etrans; eauto); eauto; try refl. i. des.
+        exploit reorder_racy_read_read; try exact RACY_UPDATE; try exact STEP_SRC; eauto; ss. i. des.
+        esplits.
+        + ss.
+        + econs 2; [|econs 1]. econs.
+          * econs. econs 2. econs; [|econs 2]; eauto. econs. econs.
+          * eauto.
+        + econs 2. econs 2. econs; [|econs 9]; eauto. econs. econs.
+          erewrite RegFile.eq_except_rmw; eauto; cycle 1.
+          * apply RegFile.eq_except_singleton.
+          * symmetry. eauto.
+        + eauto.
+        + eauto.
+        + eauto.
+        + left. eapply paco11_mon; [apply sim_stmts_nil|]; ss.
+          apply RegFun.add_add. ii. subst. eapply REGS.
+          apply RegSet.singleton_spec. eauto.
+      - (* store *)
+        right.
+        guardH ORD21.
+        apply RegSet.disjoint_add in REGS. des.
+        hexploit sim_local_write_bot; try exact LOCAL1; try exact SC;
+          try exact WF_SRC; try exact WF_TGT; try refl; eauto; try by viewtac. i. des.
+        exploit reorder_racy_read_write; try exact RACY_UPDATE; eauto. i. des.
+        esplits.
+        + ss.
+        + econs 2; [|econs 1]. econs.
+          * econs. econs 2. econs; [|econs 3]; eauto. econs.
+            erewrite RegFile.eq_except_value; cycle 2.
+            { apply RegFile.eq_except_singleton. }
+            { econs. }
+            { ii. apply RegSet.singleton_spec in LHS. subst. congr. }
+          * eauto.
+        + econs 2. econs 2. econs; [|econs 9]; eauto. econs. econs. eauto.
+        + eauto.
+        + eauto.
+        + ss.
+        + left. eapply paco11_mon; [apply sim_stmts_nil|]; ss.
+      - (* na write *)
+        inv LOCAL1. destruct ord; ss.
+      - (* racy read *)
+        right.
+        apply RegSet.disjoint_add in REGS. des.
+        exploit sim_local_racy_read; try exact LOCAL; eauto; try refl. i. des.
+        esplits.
+        + ss.
+        + econs 2; [|econs 1]. econs.
+          * econs. econs 2. econs; [|econs 9]; eauto. econs. econs.
+          * eauto.
+        + econs 2. econs 2. econs; [|econs 9]; try exact RACY_UPDATE. econs. econs.
+          erewrite RegFile.eq_except_rmw; eauto; cycle 1.
+          * apply RegFile.eq_except_singleton.
+          * symmetry. eauto.
+        + eauto.
+        + eauto.
+        + eauto.
+        + left. eapply paco11_mon; [apply sim_stmts_nil|]; ss.
+          apply RegFun.add_add. ii. subst. eapply REGS.
+          apply RegSet.singleton_spec. eauto.
+      - (* racy write *)
+        left. guardH ORD21.
+        exploit sim_local_racy_write; try exact LOCAL1; try apply RACY_UPDATE;
+          try match goal with
+              | [|- is_true (Ordering.le _ _)] => refl
+              end; eauto.
+        i. des.
+        unfold Thread.steps_failure. esplits; try refl.
+        + econs 2. econs; [|econs 10]; eauto. econs. econs.
+        + ss.
+    }
+
+    { ii. left. unfold Thread.steps_failure.
+      inv REORDER.
+      - (* load *)
+        exploit progress_read_step_cur; try exact WF_SRC; eauto. i. des.
+        exploit read_step_cur_future; try exact READ; eauto. i. des.
+        esplits.
+        + econs 2; try refl. econs.
+          * econs. econs 2. econs; [|econs 2]; eauto. econs. econs.
+          * ss.
+        + econs 2. econs; [|econs 11].
+          * econs. econs.
+            erewrite RegFile.eq_except_rmw; eauto; cycle 1.
+            { apply RegFile.eq_except_singleton. }
+            { ii. eapply REGS; eauto.
+              apply RegSet.add_spec. auto.
+            }
+          * assert (CONS: Local.promise_consistent lc2).
+            { ii. rewrite <- PROMISES, <- TVIEW in *. inv RACY_UPDATE; eauto. }
+            inv RACY_UPDATE.
+            { econs 1; eauto. }
+            { econs 2; eauto. }
+            { econs 3; eauto; try congr.
+              inv RACE. econs. rewrite <- TVIEW. ss.
+            }
+        + ss.
+      - (* store *)
+        guardH ORD21.
+        exploit (@LowerPromises.steps_promises_rel
+                   lang (Thread.mk lang (State.mk rs [Stmt.instr (Instr.store l2 v2 o2); Stmt.instr (Instr.update r1 l1 rmw1 or1 ow1)])
+                                   lc1_src sc1_src mem1_src)); s; eauto.
+        i. des. destruct e2, state. ss.
+        exploit LowerPromises.rtc_opt_promise_step_future; eauto. s. i. des. inv STATE.
+        hexploit LowerPromises.promises_rel_promise_consistent; eauto; i.
+        { inv RACY_UPDATE; eauto. }
+        hexploit LowerPromises.promises_rel_nonsynch; eauto. i.
+        exploit Thread.rtc_tau_step_future; try exact STEPS0; eauto. s. i. des.
+        exploit write_step_consistent; try exact WF2; eauto. i. des.
+        esplits.
+        + eapply rtc_n1; eauto. econs.
+          * econs. econs 2. econs; [|econs 3; eauto]. econs. econs.
+          * ss.
+        + econs 2. econs; [|econs 11].
+          * econs. econs. eauto.
+          * inv RACY_UPDATE.
+            { econs 1; eauto. }
+            { econs 2; eauto. }
+            { exploit Thread.rtc_tau_step_non_promised; try exact STEPS0; eauto. s. i. des.
+              exploit Local.program_step_non_promised; [econs 3|..]; try exact STEP; eauto. i. des.
+              econs 3; eauto; try congr.
+              inv RACE. econs. rewrite TVIEW in TS.
+              inv STEP. ss.
+              apply TimeFacts.join_spec_lt; auto.
+              unfold TimeMap.singleton, Loc.LocFun.add, Loc.LocFun.init, Loc.LocFun.find. condtac; ss.
+              eapply TimeFacts.le_lt_lt; eauto. apply Time.bot_spec.
+            }
+        + ss.
+    }
+  }
 Grab Existential Variables.
 { econs 2. }
 { econs. econs 3. }
@@ -358,38 +539,73 @@ Proof.
   pcofix CIH. i. pfold. ii. ss. splits; ss; ii.
   - inv TERMINAL_TGT. inv PR; ss.
   - exploit sim_update_mon; eauto. i.
-    inversion x0. subst. i.
-    exploit (progress_program_step_non_update
-               (RegFun.add r1 (fst (RegFile.eval_rmw rs rmw1 vr1)) rs) i2 nil); eauto.
-    { inv REORDER; ss. }
-    i. des.
-    destruct th2. exploit sim_update_step; eauto.
-    { rewrite RMW in *. ss. econs 2. eauto. }
-    i. des; eauto.
-    + exploit Thread.program_step_promises_bot; eauto. s. i.
-      exploit Thread.rtc_tau_step_future; eauto. s. i. des.
-      exploit Thread.opt_step_future; eauto. s. i. des.
-      exploit Thread.program_step_future; eauto. s. i. des.
-      punfold SIM. exploit SIM; try apply SC3; eauto; try refl.
-      { exploit Thread.program_step_promises_bot; eauto. s. i.
-        eapply Local.bot_promise_consistent; eauto. }
-      s. i. des.
-      exploit PROMISES; eauto. i. des.
-      * left.
-        unfold Thread.steps_failure in *. des.
-        esplits; [|eauto|]; ss.
-        etrans; eauto. etrans; [|eauto].
-        inv STEP_SRC; eauto. econs 2; eauto. econs.
-        { econs. eauto. }
-        { etrans; eauto.
-          destruct e; by inv STEP; inv STATE; inv INSTR; inv REORDER. }
-      * right. esplits; [|eauto].
-        etrans; eauto. etrans; [|eauto].
-        inv STEP_SRC; eauto. econs 2; eauto. econs.
-        { econs. eauto. }
-        { etrans; eauto.
-          destruct e; by inv STEP; inv STATE; inv INSTR; inv REORDER. }
-    + inv SIM. inv STEP; inv STATE.
+    inversion x0.
+    { subst. i.
+      exploit (progress_program_step_non_update
+                 (RegFun.add r1 (fst (RegFile.eval_rmw rs rmw1 vr1)) rs) i2 nil); eauto.
+      { inv REORDER; ss. }
+      i. des.
+      destruct th2. exploit sim_update_step; eauto.
+      { rewrite RMW in *. ss. econs 2. eauto. }
+      i. des; eauto.
+      + exploit Thread.program_step_promises_bot; eauto. s. i.
+        exploit Thread.rtc_tau_step_future; eauto. s. i. des.
+        exploit Thread.opt_step_future; eauto. s. i. des.
+        exploit Thread.program_step_future; eauto. s. i. des.
+        punfold SIM. exploit SIM; try apply SC3; eauto; try refl.
+        { exploit Thread.program_step_promises_bot; eauto. s. i.
+          eapply Local.bot_promise_consistent; eauto. }
+        s. i. des.
+        exploit PROMISES; eauto. i. des.
+        * left.
+          unfold Thread.steps_failure in *. des.
+          esplits; [|eauto|]; ss.
+          etrans; eauto. etrans; [|eauto].
+          inv STEP_SRC; eauto. econs 2; eauto. econs.
+          { econs. eauto. }
+          { etrans; eauto.
+            destruct e; by inv STEP; inv STATE; inv INSTR; inv REORDER. }
+        * right. esplits; [|eauto].
+          etrans; eauto. etrans; [|eauto].
+          inv STEP_SRC; eauto. econs 2; eauto. econs.
+          { econs. eauto. }
+          { etrans; eauto.
+            destruct e; by inv STEP; inv STATE; inv INSTR; inv REORDER. }
+      + inv SIM;  inv STEP; inv STATE.
+    }
+    { subst. i.
+      exploit (progress_program_step_non_update
+                 (RegFun.add r1 (fst (RegFile.eval_rmw rs rmw1 vr1)) rs) i2 nil); eauto.
+      { inv REORDER; ss. }
+      i. des.
+      destruct th2. exploit sim_update_step; eauto.
+      { rewrite RMW in *. ss. econs 2. eauto. }
+      i. des; eauto.
+      + exploit Thread.program_step_promises_bot; eauto. s. i.
+        exploit Thread.rtc_tau_step_future; eauto. s. i. des.
+        exploit Thread.opt_step_future; eauto. s. i. des.
+        exploit Thread.program_step_future; eauto. s. i. des.
+        punfold SIM. exploit SIM; try apply SC3; eauto; try refl.
+        { exploit Thread.program_step_promises_bot; eauto. s. i.
+          eapply Local.bot_promise_consistent; eauto. }
+        s. i. des.
+        exploit PROMISES; eauto. i. des.
+        * left.
+          unfold Thread.steps_failure in *. des.
+          esplits; [|eauto|]; ss.
+          etrans; eauto. etrans; [|eauto].
+          inv STEP_SRC; eauto. econs 2; eauto. econs.
+          { econs. eauto. }
+          { etrans; eauto.
+            destruct e; by inv STEP; inv STATE; inv INSTR; inv REORDER. }
+        * right. esplits; [|eauto].
+          etrans; eauto. etrans; [|eauto].
+          inv STEP_SRC; eauto. econs 2; eauto. econs.
+          { econs. eauto. }
+          { etrans; eauto.
+            destruct e; by inv STEP; inv STATE; inv INSTR; inv REORDER. }
+      + inv SIM; inv STEP; inv STATE.
+    }
   - exploit sim_update_mon; eauto. i. des.
     exploit sim_update_step; eauto. i. des; eauto.
     + right. esplits; eauto.
